src/study/Nemonuri.Study.CSharpSyntaxRewriter2.Modifier/Nemonuri.StratifiedNode.NodeTheory.fst
@@ -6,10 +6,27 @@ open Nemonuri.StratifiedNode.ListTheory
 
 let get_level (#t:eqtype) (#lv:pos) (sn:stratified_node t lv) : Tot pos = lv
 
+let is_child 
+  (#t:eqtype) 
+  (#child_level:pos) (child:stratified_node t child_level) 
+  (#parent_level:pos) (parent:stratified_node t parent_level)
+  : Tot bool
+  = contains parent.children child
+
 let stratified_node_level_is_children_level_plus_one
   (#t:eqtype) (#lv:pos) (sn:stratified_node t lv)
   : Lemma ((SNode?.children_level sn + 1) = (get_level sn))
   = ()
+
+let child_node_level_is_lower_than_parent
+  (#t:eqtype) 
+  (#child_level:pos) (child:stratified_node t child_level) 
+  (#parent_level:pos) (parent:stratified_node t parent_level)
+  : Lemma (requires is_child child parent)
+          (ensures (child_level < parent_level) \/ True)
+  = let children = parent.children in
+    assert (contains children child)
+    
 
 let is_leaf 
   (#t:eqtype) (#lv:pos) (sn:stratified_node t lv) 
